$$
\begin{align}
{L(\pi)}&=\begin{pmatrix}n\\y\end{pmatrix}\pi^y\ast(1-\pi)^{n-y}\\
\ln{L(\pi)}&=\ln{(\frac{n!}{y!(n-y)!})}+y\ln\pi+(n-1)\ln(1-\pi)\\
1.\sqcup{(\pi)}&=\frac{\sigma\ln{L(\pi)}}{\sigma\pi}=\frac{y-n\pi}{\pi(1-\pi)}\\
2.\frac{\sigma^2\ln{L(\pi)}}{\sigma^2\pi}&=\frac{2y\pi-y-n\pi^2}{\pi^2(1-\pi)^2}\\
I(\pi)&=-E\left[\frac{2y\pi-y-n\pi^2}{\pi^2(1-\pi)^2}\right]=-E\left[\frac{2Y\pi-Y-n\pi^2}{\pi^2(1-\pi)^2}\right]=\frac{n}{\pi(1-\pi)}\\
3.S(\pi)&=\frac{\sqcup(\pi)^2}{I(\pi)} \quad\text{Let $\hat{\pi}=\frac{y}{n}(MLE)$}\\
\Longrightarrow S(\pi_0)=\frac{(\hat{\pi}-\pi_0)^2}{\frac{\pi_0()}{}}
\end{align}

$$